lithium/adequacy.v
@@ -1,0 +1,181 @@
+From iris.algebra Require Import csum excl auth cmra_big_op gmap.
+(*From iris.base_logic.lib Require Import ghost_map.*)
+From VST.veric Require Import SequentialClight.
+From VST.lithium Require Export type.
+From VST.lithium Require Import programs function bytes globals int fixpoint.
+Set Default Proof Using "Type".
+
+(* Class typePreG Σ := PreTypeG {
+  type_invG                      :: invGpreS Σ;
+  type_heap_heap_inG             :: heapGpreS Σ;
+(*  type_heap_alloc_meta_map_inG  :: ghost_mapG Σ alloc_id (Z * nat * alloc_kind);
+  type_heap_alloc_alive_map_inG  :: ghost_mapG Σ alloc_id bool;
+  type_heap_fntbl_inG            :: ghost_mapG Σ addr function; *)
+}.
+
+Definition typeΣ : gFunctors :=
+  #[invΣ;
+   GFunctor (constRF (authR heapUR));
+   ghost_mapΣ alloc_id (Z * nat * alloc_kind);
+   ghost_mapΣ alloc_id bool;
+   ghost_mapΣ addr function].
+Global Instance subG_typePreG {Σ} : subG typeΣ Σ → typePreG Σ.
+Proof. solve_inG. Qed. *)
+
+Definition main_type `{!typeG Σ} {cs : compspecs} (P : iProp Σ) : {A : TypeTree & (dtfr(Σ := Σ) A → function.fn_params)%type} :=
+  existT (ConstType unit) (fn(∀ () : (); P) → ∃ () : (), int.int tint; True).
+
+Global Instance VST_typeG `{!VSTGS OK_ty Σ} : typeG Σ := TypeG _ _.
+
+Definition typed_func `{!VSTGS OK_ty Σ} (V: varspecs) {C: compspecs}
+  (t : {A : TypeTree & (dtfr A → function.fn_params)%type})
+  (ge: Genv.t Clight.fundef Ctypes.type) (id: ident) (f: function) :=
+  semax_body_params_ok f = true /\
+      Forall
+         (fun it : ident * Ctypes.type =>
+          complete_type cenv_cs (snd it) =
+          true) (fn_vars f) /\
+       var_sizes_ok (f.(fn_vars)) /\
+       ∃ b, Genv.find_symbol ge id = Some b /\ Genv.find_funct_ptr ge b = Some (Internal f) /\
+      ∀ OK_spec : ext_spec OK_ty,
+      (* at least need function pointers *) ⊢ (Vptr b Ptrofs.zero) ◁ᵥ (b, 0%Z) @ function_ptr t.
+
+(* RefinedC assumes that typechecking main implicitly typechecks all functions it calls.
+   Can we do that too, or do we need to say that each function meets its specified type
+   (and convert G to a list of types for each function)? *)
+
+(* just main *)
+Definition typed_prog `{!VSTGS OK_ty Σ} {OK_spec : ext_spec OK_ty} {C: compspecs}
+       (prog: Clight.program) (ora: OK_ty) (V: varspecs) : Prop :=
+compute_list_norepet (prog_defs_names prog) = true  /\
+all_initializers_aligned prog /\
+Maps.PTree.elements cenv_cs = Maps.PTree.elements (prog_comp_env prog) /\
+(*typed_func V G (Genv.globalenv prog) (prog_funct prog) G /\*)
+match_globvars (prog_vars prog) V = true /\
+∃ f, typed_func V (main_type emp) (Genv.globalenv (program_of_program prog)) prog.(prog_main) f.
+
+(* Definition typed_prog `{!VSTGS OK_ty Σ} {OK_spec : ext_spec OK_ty} {C: compspecs}
+       (prog: program) (ora: OK_ty) (V: varspecs) (G: funspecs) : Prop :=
+compute_list_norepet (prog_defs_names prog) = true  /\
+all_initializers_aligned prog /\
+Maps.PTree.elements cenv_cs = Maps.PTree.elements (prog_comp_env prog) /\
+typed_func V G (Genv.globalenv prog) (prog_funct prog) G /\
+match_globvars (prog_vars prog) V = true /\
+match find_id prog.(prog_main) G with
+| Some s => exists post,
+      s = main_spec_ext' prog ora post
+| None => False
+end. *)
+
+
+(*[∗ list] main ∈ thread_mains, ∃ P, main ◁ᵥ main @ function_ptr (main_type P) ∗ P*)
+
+(** * The main adequacy lemma *)
+Lemma refinedc_adequacy Σ `{!VSTGpreS OK_ty Σ} {Espec : forall `{VSTGS OK_ty Σ}, ext_spec OK_ty} {dryspec : ext_spec OK_ty} (initial_oracle: OK_ty)
+     (EXIT: forall `{!VSTGS OK_ty Σ}, semax_prog.postcondition_allows_exit Espec tint)
+     (Hdry : forall `{!VSTGS OK_ty Σ}, ext_spec_entails Espec dryspec)
+     prog V m :
+     (forall {HH : VSTGS OK_ty Σ}, exists CS: compspecs, typed_prog(OK_spec := Espec) prog initial_oracle V) ->
+     Genv.init_mem prog = Some m ->
+     exists b, exists q,
+       Genv.find_symbol (Genv.globalenv prog) (prog_main prog) = Some b /\
+       semantics.initial_core (Clight_core.cl_core_sem (globalenv prog))
+           0 m q m (Vptr b Ptrofs.zero) nil /\
+       forall n,
+        @step_lemmas.dry_safeN _ _ _ OK_ty (genv_symb_injective)
+            (Clight_core.cl_core_sem (globalenv prog))
+            dryspec
+            (Build_genv (Genv.globalenv prog) (prog_comp_env prog))
+             n initial_oracle q m.
+Proof.
+  
+Qed.
+
+(*Lemma refinedc_adequacy Σ `{!typePreG Σ} (thread_mains : list loc) (fns : gmap addr function) (gls : list loc) (gvs : list val.val) n t2 σ2 κs hs σ:
+  alloc_new_blocks initial_heap_state GlobalAlloc gls gvs hs →
+  σ = {| st_heap := hs; st_fntbl := fns; |} →
+  (∀ {HtypeG : typeG Σ}, ∃ gl gt,
+  let Hglobals : globalG Σ := {| global_locs := gl; global_initialized_types := gt; |} in
+    ([∗ list] l; v ∈ gls; gvs, l ↦ v) -∗
+    ([∗ map] k↦qs∈fns, fntbl_entry (fn_loc k) qs) ={⊤}=∗
+      [∗ list] main ∈ thread_mains, ∃ P, main ◁ᵥ main @ function_ptr (main_type P) ∗ P) →
+  nsteps (Λ := c_lang) n (initial_prog <$> thread_mains, σ) κs (t2, σ2) →
+  ∀ e2, e2 ∈ t2 → not_stuck e2 σ2.
+Proof.
+  move => Hnew -> Hwp. apply: wp_strong_adequacy. move => ?.
+  set h := to_heapUR ∅.
+  iMod (own_alloc (● h ⋅ ◯ h)) as (γh) "[Hh _]" => //.
+  { apply auth_both_valid_discrete. split => //. }
+  iMod (ghost_map_alloc fns) as (γf) "[Hf Hfm]".
+  iMod (ghost_map_alloc_empty (V:=(Z * nat * alloc_kind))) as (γr) "Hr".
+  iMod (ghost_map_alloc_empty (V:=bool)) as (γs) "Hs".
+  set (HheapG := HeapG _ _ γh _ γr _ γs _ γf).
+  set (HrefinedCG := RefinedCG _ _ HheapG).
+  set (HtypeG := TypeG _ HrefinedCG).
+  move: (Hwp HtypeG) => {Hwp} [gl [gt]].
+  set (Hglobals := {| global_locs := gl; global_initialized_types := gt; |}).
+  move => Hwp.
+  iMod (heap_alloc_new_blocks_upd with "[Hh Hr Hs]") as "[Hctx Hmt]" => //. {
+    rewrite /heap_state_ctx /alloc_meta_ctx /to_alloc_meta_map /alloc_alive_ctx /to_alloc_alive_map !fmap_empty.
+    by iFrame.
+  }
+  rewrite big_sepL2_sep. iDestruct "Hmt" as "[Hmt Hfree]".
+  iAssert (|==> [∗ map] k↦qs ∈ fns, fntbl_entry (fn_loc k) qs)%I with "[Hfm]" as ">Hfm". {
+    iApply big_sepM_bupd. iApply (big_sepM_impl with "Hfm").
+    iIntros "!>" (???) "Hm". rewrite fntbl_entry_eq.
+    iExists _. iSplitR; [done|]. by iApply ghost_map_elem_persist.
+  }
+  iMod (Hwp with "Hmt Hfm") as "Hmains".
+
+  iModIntro. iExists _, (replicate (length thread_mains) (λ _, True%I)), _, _.
+  iSplitL "Hctx Hf"; last first. 1: iSplitL "Hmains".
+  - rewrite big_sepL2_fmap_l. iApply big_sepL2_replicate_r; [done|]. iApply (big_sepL_impl with "Hmains").
+    iIntros "!#" (? main ?); iDestruct 1 as (P) "[Hmain HP]".
+    iApply (type_call with "[-]"). 2: { by iIntros (??) "??". }
+    iApply type_val. iApply type_val_context.
+    iExists (main @ function_ptr (main_type P))%I => /=. iFrame => /=.
+    iApply type_call_fnptr. iIntros "_". iExists () => /=. iFrame. by iIntros (v []) "Hv" => /=.
+  - iFrame. iIntros (?? _ _ ?) "_ _ _". iApply fupd_mask_intro_discard => //. iPureIntro. by eauto.
+  - by iFrame.
+Qed.
+
+(** * Helper functions for using the adequacy lemma *)
+Definition fn_lists_to_fns (addrs : list addr) (fns : list function) : gmap addr function :=
+  list_to_map (zip addrs fns).
+
+Lemma fn_lists_to_fns_cons `{!refinedcG Σ} addr fn addrs fns :
+  length addrs = length fns →
+  addr ∉ addrs →
+  ([∗ map] k↦qs ∈ fn_lists_to_fns (addr :: addrs) (fn :: fns), fntbl_entry (fn_loc k) qs) -∗
+  fntbl_entry (ProvFnPtr, addr) fn ∗ ([∗ map] k↦qs ∈ fn_lists_to_fns addrs fns, fntbl_entry (fn_loc k) qs).
+Proof.
+  move => Hnotin ?.
+  rewrite /fn_lists_to_fns /= big_sepM_insert. { by iIntros "?". }
+  apply not_elem_of_list_to_map_1. rewrite fst_zip => //; lia.
+Qed.*)
+
+(** * Tactics for solving conditions in an adequacy proof *)
+
+Ltac adequacy_intro_parameter :=
+  repeat lazymatch goal with
+         | |- ∀ _ : (), _ => case
+         | |- ∀ _ : (_ * _), _ => case
+         | |- ∀ _ : _, _ => move => ?
+         end.
+
+Ltac adequacy_unfold_equiv :=
+  lazymatch goal with
+  | |- type_fixpoint _ _ ≡ type_fixpoint _ _ => apply: type_fixpoint_proper; [|move => ??]
+  | |- ty_own_val _ _ ≡ ty_own_val _ _ => unfold ty_own_val => /=
+  | |-  _ =@{struct_layout} _ => apply: struct_layout_eq
+  end.
+
+Ltac adequacy_solve_equiv unfold_tac :=
+  first [ eassumption | fast_reflexivity | unfold_type_equiv | adequacy_unfold_equiv | f_contractive | f_equiv' | reflexivity | progress unfold_tac ].
+
+Ltac adequacy_solve_typed_function lemma unfold_tac :=
+  iApply typed_function_equiv; [
+    done |
+    adequacy_intro_parameter => /=; repeat (constructor; [done|]); by constructor |
+    | iApply lemma => //; iExists _; repeat iSplit => //];
+    adequacy_intro_parameter => /=; eexists eq_refl => /=; split_and!; [..|adequacy_intro_parameter => /=; split_and!];  repeat adequacy_solve_equiv unfold_tac.
